Update local steps w.r.t. reserve messages

src/model/Global.v
@@ -13,7 +13,6 @@ Require Import Time.
 Require Import View.
 Require Import BoolMap.
 Require Import Promises.
-Require Import Reserves.
 Require Import Cell.
 Require Import Memory.
 
@@ -24,22 +23,17 @@ Module Global.
   Structure t := mk {
     sc: TimeMap.t;
     promises: BoolMap.t;
-    reserves: BoolMap.t;
     memory: Memory.t;
   }.
 
-  Definition init := mk TimeMap.bot BoolMap.bot BoolMap.bot Memory.init.
-
-  Definition fully_reserved (gl: t): t :=
-    mk (sc gl) (promises gl) BoolMap.top (memory gl).
-  #[export] Hint Unfold fully_reserved: core.
+  Definition init := mk TimeMap.bot BoolMap.bot Memory.init.
 
   Variant wf (gl: t): Prop :=
   | wf_intro
       (SC_CLOSED: Memory.closed_timemap (sc gl) (memory gl))
       (MEM_CLOSED: Memory.closed (memory gl))
   .
-  #[export] Hint Constructors wf: core.
+  #[global] Hint Constructors wf: core.
 
   Lemma init_wf: wf init.
   Proof.
@@ -49,12 +43,22 @@ Module Global.
     - apply Memory.init_closed.
   Qed.
 
-  Lemma fully_reserved_wf
+  Variant cap (gl gl_cap: t): Prop :=
+    | cap_intro
+        (SC: sc gl = sc gl_cap)
+        (PROMISES: promises gl = promises gl_cap)
+        (MEMORY: Memory.cap (memory gl) (memory gl_cap))
+  .
+  #[global] Hint Constructors cap: core.
+
+  Lemma cap_exists
         gl
         (WF: wf gl):
-    wf (fully_reserved gl).
+    exists gl_cap, cap gl gl_cap.
   Proof.
-    inv WF. econs; ss.
+    destruct gl.
+    exploit Memory.cap_exists; try apply WF. s. i. des.
+    eexists (mk _ _ _). econs; s; eauto.
   Qed.
 
   Variant future (gl1 gl2: t): Prop :=
@@ -62,7 +66,7 @@ Module Global.
       (SC: TimeMap.le (sc gl1) (sc gl2))
       (MEMORY: Memory.future (memory gl1) (memory gl2))
   .
-  #[export] Hint Constructors future: core.
+  #[global] Hint Constructors future: core.
 
   Global Program Instance future_PreOrder: PreOrder future.
   Next Obligation.
@@ -71,5 +75,39 @@ Module Global.
   Next Obligation.
     ii. destruct x, y, z. inv H. inv H0. ss.
     econs; etrans; eauto.
+  Qed.
+
+  Variant le (gl1 gl2: t): Prop :=
+    | le_intro
+        (SC: TimeMap.le (sc gl1) (sc gl2))
+        (MEMORY: Memory.messages_le (memory gl1) (memory gl2))
+  .
+  #[global] Hint Constructors le: core.
+
+  Global Program Instance le_PreOrder: PreOrder le.
+  Next Obligation.
+    ii. econs; refl.
+  Qed.
+  Next Obligation.
+    ii. inv H. inv H0. econs; etrans; eauto.
+  Qed.
+
+  Lemma future_le
+    gl1 gl2
+    (FUTURE: future gl1 gl2):
+    le gl1 gl2.
+  Proof.
+    inv FUTURE. econs; ss.
+    eauto using Memory.future_messages_le.
+  Qed.
+
+  Lemma cap_le
+    gl gl_cap
+    (CAP: cap gl gl_cap):
+    le gl gl_cap.
+  Proof.
+    destruct gl, gl_cap. inv CAP. ss. subst.
+    econs; s; try refl.
+    eauto using Memory.cap_messages_le.
   Qed.
 End Global.
